ExistentialRules/ChaseSequence/Nontermination/SparseSubderivationGenerator.lean
@@ -252,6 +252,52 @@ theorem densify_generator.childTrees_empty_of_next_none {β : Type u}
     exact maximal _
   . simp
 
+/-- Given any `DensifiedResult`, if we iterate the `densify_generator` n times, where n is the length of the list in the second component, then we obtain a densified result where the first component is unchanged but the second component is the empty list. Intuitively, we have then iterated over exactly the list elements in the second component. -/
+theorem densify_generator.original_generator_value_after_exhausting_list {β : Type u}
+    {td : TreeDerivation obs rules} {generator : β -> Option β} {mapper : β -> NodeWithAddress td} :
+    ∀ dr : DensifiedResult β td, (·.bind (td.densify_generator generator mapper)).repeat_fun dr.snd.length (some dr) = some ⟨dr.fst, []⟩ := by
+  intro dr
+  induction eq : dr.snd generalizing dr with
+  | nil => rw [List.length_nil, Function.repeat_zero]; grind
+  | cons hd tl ih =>
+    rw [List.length_cons, Function.repeat_add, Function.repeat_once, Option.bind_some]
+    have dr_eq : dr = ⟨dr.fst, hd::tl⟩ := by grind
+    rw [dr_eq]
+    simp only [densify_generator]
+    apply ih
+    rfl
+
+/-- Every value that can be reached by iterating the original generator can also be reached by iterating the densified version (but the number of iterations can and will most of the time be different). -/
+theorem mem_densify_generator_of_mem_generator {β : Type u}
+    (td : TreeDerivation obs rules) (generator : β -> Option β) (mapper : β -> NodeWithAddress td)
+    (start : β) : ∀ n, ∃ m, (·.bind (td.densify_generator generator mapper)).repeat_fun m (some ⟨start, []⟩) = ((·.bind generator).repeat_fun n (some start)).map (fun b' => ⟨b', []⟩) := by
+  intro n; induction n with
+  | zero => exists 0
+  | succ n ih =>
+    rcases ih with ⟨m, ih⟩
+    cases eq_next : (·.bind generator).repeat_fun n.succ (some start) with
+    | none =>
+      exists m + 1; rw [Option.map_none]
+      rw [Function.repeat_add, Function.repeat_once, ← Function.repeat_swap_one, ih]
+      rw [Option.bind_eq_none_iff]
+      intro val val_eq; rw [Option.map_eq_some_iff] at val_eq; rcases val_eq with ⟨b, b_eq, val_eq⟩
+      simp only [densify_generator, ← val_eq]
+      rw [Function.repeat_succ, b_eq, Option.bind_some] at eq_next
+      rw [eq_next]
+      simp
+    | some next =>
+      cases eq_current : (·.bind generator).repeat_fun n (some start) with
+      | none => rw [Function.repeat_succ, eq_current] at eq_next; simp at eq_next
+      | some current =>
+        exists m + ((mapper current).nodes_to (mapper next)).length.succ
+        rw [Option.map_some]
+        rw [Function.repeat_add, Function.repeat_swap, Function.repeat_succ, (Option.bind · (td.densify_generator generator mapper)).repeat_swap_one]
+        rw [ih, eq_current]
+        simp only [Option.map_some, Option.bind_some, densify_generator]
+        suffices generator current = next by
+          rw [this]; exact densify_generator.original_generator_value_after_exhausting_list ⟨next, (mapper current).nodes_to (mapper next)⟩
+        rw [← eq_next, Function.repeat_succ, eq_current]; simp
+
 /-- A version of `densify_generator` that works only on `wellFormed` `DensifiedResult`s. -/
 def densify_generator' {β : Type u} (td : TreeDerivation obs rules) (generator : β -> Option β) (mapper : β -> NodeWithAddress td)
     (next_is_succ : ∀ b, ∀ b' ∈ generator b, mapper b ≺ mapper b')
@@ -264,6 +310,32 @@ def densify_generator' {β : Type u} (td : TreeDerivation obs rules) (generator 
 def densify_mapper' (td : TreeDerivation obs rules) (mapper : β -> NodeWithAddress td)
     (dr : {dr : DensifiedResult β td // dr.wellFormed mapper}) : NodeWithAddress td :=
   densify_mapper td mapper dr.val
+
+/-- Rpeating `densify_generator'` is not different than repeating `densify_generator` except that we need to isolate the value of the subtype. -/
+theorem densify_generator'_eq_densify_generator {β : Type u}
+    {td : TreeDerivation obs rules} {generator : β -> Option β} {mapper : β -> NodeWithAddress td}
+    {next_is_succ : ∀ b, ∀ b' ∈ generator b, mapper b ≺ mapper b'}
+    {dr : {dr : DensifiedResult β td // dr.wellFormed mapper}} :
+    ∀ n, ((·.bind (td.densify_generator' generator mapper next_is_succ)).repeat_fun n (some dr)).map Subtype.val =
+      ((·.bind (td.densify_generator generator mapper)).repeat_fun n (some dr.val)) := by
+  intro n; induction n with
+  | zero => simp [Function.repeat_zero]
+  | succ n ih =>
+    rw [Function.repeat_succ]
+    conv => right; rw [Function.repeat_succ]
+    rw [← ih]
+    cases (·.bind (td.densify_generator' generator mapper next_is_succ)).repeat_fun n (some dr) <;> simp [densify_generator']
+
+/-- Applying `densify_mapper'` after any number of repetitions of `densify_generator'` is the same as applyign `densify_mapper` after repeating `densify_generator` for the same number of iterations. -/
+theorem densify'_eq_densify {β : Type u}
+    {td : TreeDerivation obs rules} {generator : β -> Option β} {mapper : β -> NodeWithAddress td}
+    {next_is_succ : ∀ b, ∀ b' ∈ generator b, mapper b ≺ mapper b'}
+    {dr : {dr : DensifiedResult β td // dr.wellFormed mapper}} :
+    ∀ n, ((·.bind (td.densify_generator' generator mapper next_is_succ)).repeat_fun n (some dr)).map (td.densify_mapper' mapper) =
+      ((·.bind (td.densify_generator generator mapper)).repeat_fun n (some dr.val)).map (td.densify_mapper mapper) := by
+  intro n
+  rw [← densify_generator'_eq_densify_generator (next_is_succ := next_is_succ)]
+  cases (·.bind (td.densify_generator' generator mapper next_is_succ)).repeat_fun n (some dr) <;> simp [densify_mapper']
 
 /-- Given a sparse generator function, uses the original `TreeDerivation.generate_subderivation` function together with `densify_generator` and `densify_mapper` to generate a `ChaseDerivation` that corresponds to a branch in the tree. -/
 def generate_subderivation_from_sparse {β : Type u} (td : TreeDerivation obs rules)
@@ -295,6 +367,41 @@ public def generate_subderivation_from_sparse_of_total_generator {β : Type u} (
   td.generate_subderivation_from_sparse start (Option.some ∘ generator) mapper
     (by intro b _ eq; rw [Function.comp_apply, Option.mem_def, Option.some_inj] at eq; rw [← eq]; exact next_is_succ b)
     (by simp)
+
+/-- `generate_subderivation_from_sparse_of_total_generator` produces a tree branch because underneath it uses `TreeDerivation.generate_subderivation`, which already has this property. -/
+public theorem generate_subderivation_from_sparse_of_total_generator_mem_branches
+    {β : Type u} {td : TreeDerivation obs rules}
+    {start : β} {generator : β -> β} {mapper : β -> NodeWithAddress td}
+    {next_is_succ : ∀ b, mapper b ≺ mapper (generator b)}
+    (start_eq : mapper start = NodeWithAddress.root td) :
+    (td.generate_subderivation_from_sparse_of_total_generator start generator mapper next_is_succ)
+      ∈ td.branches := by
+  unfold generate_subderivation_from_sparse_of_total_generator generate_subderivation_from_sparse
+  apply generate_subderivation_mem_branches
+  simp only [densify_mapper', densify_mapper, List.headD_nil]
+  exact start_eq
+
+/-- Every node that is part of the original generator also occurs in the derivation produces by the densified version. -/
+public theorem mem_generate_subderivation_from_sparse_of_total_generator_of_mem_original_generator
+    {β : Type u} {td : TreeDerivation obs rules}
+    {start : β} {generator : β -> β} {mapper : β -> NodeWithAddress td}
+    {next_is_succ : ∀ b, mapper b ≺ mapper (generator b)} :
+    ∀ b ∈ InfiniteList.iterate start generator, (mapper b).node ∈
+      (td.generate_subderivation_from_sparse_of_total_generator start generator mapper next_is_succ) := by
+  intro b b_mem
+  simp only [InfiniteList.mem_iff, InfiniteList.get_iterate] at b_mem
+  rcases b_mem with ⟨n, b_mem⟩
+  simp only [generate_subderivation_from_sparse_of_total_generator, generate_subderivation_from_sparse]
+  rw [TreeDerivation.mem_generate_subderivation]
+  rcases mem_densify_generator_of_mem_generator td (Option.some ∘ generator) mapper start n with ⟨m, b_mem'⟩
+  exists m
+  rw [densify'_eq_densify, b_mem']
+  suffices (·.bind (Option.some ∘ generator)).repeat_fun n (some start) = some b by rw [this]; simp [densify_mapper]
+  suffices ∀ n, (·.bind (Option.some ∘ generator)).repeat_fun n (some start) = some (generator.repeat_fun n start) by rw [this, b_mem]
+  intro n
+  induction n with
+  | zero => simp [Function.repeat_zero]
+  | succ n ih => rw [Function.repeat_succ, ih, Function.repeat_succ]; simp
 
 end TreeDerivation
 
